lib/zoo_std/mutex.mli
@@ -4,8 +4,12 @@ type t =
 val create :
   unit -> t
 
+val create_lock :
+  unit -> t
+
 val lock :
   t -> unit
+
 val unlock :
   t -> unit
 
