theories/zoo_std/mutex__opaque.v
@@ -2,6 +2,7 @@ From zoo_std Require Import
   mutex__code.
 
 #[global] Opaque mutex_create.
+#[global] Opaque mutex_create_lock.
 #[global] Opaque mutex_lock.
 #[global] Opaque mutex_unlock.
 #[global] Opaque mutex_synchronize.
